UnificationTests.thy
@@ -6,9 +6,11 @@ begin
 
 ML_file \<open>Test.ML\<close>
 ML\<open>open Test\<close>
-ML\<open>val hint_unif = Fou.first_order_unify_h
-   val std_unif = Fou.first_order_unify\<close>
+ML\<open>val hint_unif = HUnif.first_order_unify_h
+   val std_unif = HUnif.first_order_unify
+   val ctxt = Context.the_generic_context\<close>
 
+(*
 (* Symmetry *)
 ML\<open>test_group symmetry std_unif "Free/Var" free_var_gen\<close>
 ML\<open>test_group symmetry hint_unif "Free/Var" free_var_gen\<close>
@@ -43,11 +45,6 @@ ML\<open>test_group sigma_unifies_vars_replaced hint_unif "Free/Var" free_var_ge
 ML\<open>test_group occurs_check std_unif "Var only" var_gen\<close>
 ML\<open>test_group occurs_check hint_unif "Var only" var_gen\<close>
 
-(* non-unifiable Var-free terms *)
-ML\<open>test_group non_unif std_unif "Free only" free_gen\<close>
-ML\<open>test_group non_unif hint_unif "Free only" free_gen\<close>
-ML\<open>test_group non_unif_rev std_unif "Free only" free_gen\<close>
-ML\<open>test_group non_unif_rev hint_unif "Free only" free_gen\<close>
 
 (** unifiability tests **)
 (* Unification of identical terms *)
@@ -64,7 +61,7 @@ ML\<open>test_group unif_vars_replaced hint_unif "Free/Var" free_var_gen\<close>
 
 (** manual tests with Var/Free and TVar/TFree **)
 (* should unify, using std_unif *)
-ML\<open>list_pos @{context} std_unif "Var/Free, TVar/TFree combinations unify"
+ML\<open>list_pos (ctxt ()) std_unif "Var/Free, TVar/TFree combinations unify"
   [(Var(("A",0),TVar(("'a",0),[])),Free("A",TFree("'a",[]))),
    (Var(("A",0),TVar(("'a",0),[])),Var(("A",0),TFree("'a",[]))),
    (Var(("A",0),TVar(("'a",0),[])),Var(("B",0),TVar(("'a",0),[]))),
@@ -73,7 +70,7 @@ ML\<open>list_pos @{context} std_unif "Var/Free, TVar/TFree combinations unify"
    (Free("A",TFree("'a",[])),Free("A",TVar(("'a",0),[])))]\<close>
 
 (* should unify, using hint_unif *)
-ML\<open>list_pos @{context} hint_unif "Var/Free, TVar/TFree combinations unify"
+ML\<open>list_pos (ctxt ()) hint_unif "Var/Free, TVar/TFree combinations unify"
   [(Var(("A",0),TVar(("'a",0),[])),Free("A",TFree("'a",[]))),
    (Var(("A",0),TVar(("'a",0),[])),Var(("A",0),TFree("'a",[]))),
    (Var(("A",0),TVar(("'a",0),[])),Var(("B",0),TVar(("'a",0),[]))),
@@ -82,96 +79,162 @@ ML\<open>list_pos @{context} hint_unif "Var/Free, TVar/TFree combinations unify"
    (Free("A",TFree("'a",[])),Free("A",TVar(("'a",0),[])))]\<close>
 
 (* should not unify, using std_unif *)
-ML\<open>list_neg @{context} std_unif "Different Free/TFree fails"
+ML\<open>list_neg (ctxt ()) std_unif "Different Free/TFree fails"
   [(Free("A",TFree("'a",[])),Free("A",TFree("'b",[]))),
    (Free("A",TFree("'a",[])),Free("B",TFree("'a",[])))]\<close>
 (* should not unify, using hint_unif *)
-ML\<open>list_neg @{context} hint_unif "Different Free/TFree fails"
+ML\<open>list_neg (ctxt ()) hint_unif "Different Free/TFree fails"
   [(Free("A",TFree("'a",[])),Free("A",TFree("'b",[]))),
    (Free("A",TFree("'a",[])),Free("B",TFree("'a",[])))]\<close>
-
+*)
 (** hint tests **)
+
+ML\<open>
+  (* insert after unit test to view the resulting Environment and theorem *)
+(*val (env,thm) = hint_unif (ctxt ()) (t1,t2) (Envir.empty 0);
+  pretty_env @{context} (Envir.term_env env);
+  pretty_thm @{context} thm |> pwriteln *)
+\<close>
+
+ML\<open>
+  Proofterm.oracle_proof "hello" @{term_pat "1 \<equiv> 2::nat"}
+\<close>
+
+
 
 (* non-recursive hint tests *)
 
 (*add_zero*)
-ML\<open>single_neg @{context} hint_unif "add_zero without hint"
-  (@{term_pat "5::nat"},
-   @{term_pat "?b + 0 ::nat"})\<close>
-lemma add_zero [hints]: "Y \<equiv> Z \<Longrightarrow> X \<equiv> (0::nat) \<Longrightarrow> Y + X \<equiv> Z"
+ML\<open>
+  val (t1,t2) = (@{term_pat "5::nat"}, @{term_pat "?b + 0 ::nat"});
+  single_neg (ctxt ()) hint_unif "add_zero without hint" (t1,t2)\<close>
+lemma add_zero [hints]: "Y \<equiv> Z \<Longrightarrow>  X \<equiv> (0::nat) \<Longrightarrow> Y + X \<equiv> Z"
   by simp
-ML\<open>single_pos @{context} hint_unif "add_zero with hint"
-  (@{term_pat "5::nat"},
-   @{term_pat "?b + 0 ::nat"})\<close>
+ML\<open>single_pos (ctxt ()) hint_unif "add_zero with hint" (t1,t2)\<close>
 
 (*mult_one*)
-ML\<open>single_neg @{context} hint_unif "mult_one without hint"
-  (@{term_pat "1::nat"},
-    @{term_pat "?a * ?b ::nat"})\<close>
+ML\<open>
+  val (t1,t2) = (@{term_pat "1::nat"},@{term_pat "?a * ?b ::nat"});
+  single_neg (ctxt ()) hint_unif "mult_one without hint" (t1,t2)\<close>
 lemma mult_one [hints]: "X \<equiv> 1 \<Longrightarrow> Y \<equiv> 1 \<Longrightarrow> X * Y \<equiv> (1::nat)"
   by simp
-ML\<open>single_pos @{context} hint_unif "mult_one with hint"
-  (@{term_pat "1::nat"},
-   @{term_pat "?a * ?b ::nat"})\<close>
+ML\<open>single_pos (ctxt ()) hint_unif "mult_one with hint" (t1,t2)\<close>
 
 (*id_eq*)
-ML\<open>single_neg @{context} hint_unif "id_eq without hint"
-  (@{term_pat "5::nat"},
-   @{term_pat "id ?a ::nat"})\<close>
+ML\<open>
+  val (t1,t2) = (@{term_pat "5::nat"},@{term_pat "id ?a ::nat"});
+  single_neg (ctxt ()) hint_unif "id_eq without hint" (t1,t2)\<close>
 lemma ID_EQ [hints]: "X \<equiv> Y \<Longrightarrow> id X \<equiv> Y"
   by simp
-ML\<open>single_pos @{context} hint_unif "id_eq with hint"
-  (@{term_pat "5::nat"},
-   @{term_pat "id ?a ::nat"})\<close>
+ML\<open>single_pos (ctxt ()) hint_unif "id_eq with hint" (t1,t2)\<close>
 
 (*Suc 2 = 3*)
-ML\<open>single_neg @{context} hint_unif "Suc ?x = 3 without hint"
-  (@{term_pat "Suc ?x ::nat"},
-   @{term_pat "3::nat"})\<close>
+ML\<open>
+  val (t1,t2) = (@{term_pat "Suc ?x ::nat"},@{term_pat "3::nat"});
+  single_neg (ctxt ()) hint_unif "Suc ?x = 3 without hint" (t1,t2)\<close>
 lemma suc2 [hints]: "X \<equiv> 2 \<Longrightarrow> Suc X \<equiv> 3"
   by linarith
-ML\<open>single_pos @{context} hint_unif "Suc ?x = 3 with hint"
-  (@{term_pat "Suc ?x ::nat"},
-   @{term_pat "3::nat"})\<close>
+ML\<open>single_pos (ctxt ()) hint_unif "Suc ?x = 3 with hint" (t1,t2)\<close>
 
 (*Suc x = 4, multiple matching hints, first one doesn't unify*)
 definition x_def: "x\<equiv>3::nat"
-ML\<open>single_neg @{context} hint_unif "Suc x = 4 without hint"
-  (@{term_pat "Suc x ::nat"},
-   @{term_pat "4::nat"})\<close>
+ML\<open>
+  val (t1,t2) =(@{term_pat "Suc x ::nat"},@{term_pat "4::nat"});
+  single_neg (ctxt ()) hint_unif "Suc x = 4 without hint" (t1,t2)\<close>
 lemma suc_x_4 [hints]: "Suc x \<equiv> 4"
   by (simp add:x_def)
 lemma suc3 [hints]: "X \<equiv> 3 \<Longrightarrow> Suc X \<equiv> 4"
   by linarith
-ML\<open>single_pos @{context} hint_unif "Suc x = 4 with multiple matching hints, only second one solves"
-  (@{term_pat "Suc x ::nat"},
-   @{term_pat "4::nat"})\<close>
+ML\<open>single_pos (ctxt ()) hint_unif "Suc x = 4 with multiple matching hints, only second one solves"
+  (t1,t2)\<close>
 
 (* recursive hint tests *)
 
 declare [[log_level=1000]]
 
 (*Suc (Suc 0) = 2*)
-ML\<open>single_neg @{context} hint_unif "Suc ?x = 3 without hint"
-  (@{term_pat "Suc (Suc ?X) ::nat"},
-   @{term_pat "2::nat"})\<close>
+ML\<open>
+  val (t1,t2) = (@{term_pat "Suc (Suc ?X) ::nat"},@{term_pat "2::nat"});
+  single_neg (ctxt ()) hint_unif "Suc ?x = 3 without hint" (t1,t2)\<close>
 lemma suc0 [hints]: "X \<equiv> 0 \<Longrightarrow> Suc X \<equiv> 1"
   by linarith
 lemma suc1 [hints]: "X \<equiv> 1 \<Longrightarrow> Suc X \<equiv> 2"
   by linarith
-ML\<open>single_pos @{context} hint_unif "Suc ?x = 3 with hint"
-  (@{term_pat "Suc (Suc ?X) ::nat"},
-   @{term_pat "2::nat"})\<close>
+ML\<open>single_pos (ctxt ()) hint_unif "Suc ?x = 3 with hints" (t1,t2)\<close>
 
+
+consts f :: "nat \<Rightarrow> nat" g :: "nat \<Rightarrow> nat" h :: "nat \<Rightarrow> nat"
+       a :: nat b :: nat y::nat
+
+lemma [hints] : "X \<equiv> f (g 0) \<Longrightarrow> Y \<equiv> g (f 0) \<Longrightarrow> f (g X) \<equiv> g (f Y)"
+  sorry
+ML\<open>
+  val (t1,t2) = (@{term_pat "f (g (f (g 0))) ::nat"}, @{term_pat "g (f (g (f 0))) ::nat"});
+  single_pos (ctxt ()) hint_unif "" (t1,t2);\<close>
+
+(*same hint but with premises switched*)
+consts f2 :: "nat \<Rightarrow> nat" g2 :: "nat \<Rightarrow> nat"
+lemma [hints] : "Y \<equiv> g2 (f2 0) \<Longrightarrow> X \<equiv> f2 (g2 0) \<Longrightarrow> f2 (g2 X) \<equiv> g2 (f2 Y)"
+  sorry
+ML\<open>
+  val (t1,t2) = (@{term_pat "f2 (g2 (f2 (g2 0))) ::nat"}, @{term_pat "g2 (f2 (g2 (f2 0))) ::nat"});
+  single_pos (ctxt ()) hint_unif "" (t1,t2);\<close>
+
+lemma [hints]: "Y \<equiv> f X \<Longrightarrow> X \<equiv> f (g 0) \<Longrightarrow>  f (g X) \<equiv> g (f Y)"
+  sorry
+ML\<open>
+  val (t1,t2) = (@{term_pat "f (g (f (g 0))) ::nat"}, @{term_pat "g (f (f (f (g 0)))) ::nat"});
+  single_pos (ctxt ()) hint_unif "" (t1,t2);\<close>
+
+(*same hint but with premises switched*)
+lemma [hints]: "X \<equiv> f2 (g2 0) \<Longrightarrow> Y \<equiv> f2 X \<Longrightarrow>  f2 (g2 X) \<equiv> g2 (f2 Y)"
+  sorry
+ML\<open>
+  val (t1,t2) = (@{term_pat "f2 (g2 (f2 (g2 0))) ::nat"}, @{term_pat "g2 (f2 (f2 (f2 (g2 0)))) ::nat"});
+  single_pos (ctxt ()) hint_unif "" (t1,t2);\<close>
+
+(*recursive calls with encapsulated hints*)
+lemma [hints]:"X \<equiv> f \<Longrightarrow> X a \<equiv> X b"
+  sorry
+
+lemma [hints]:"X \<equiv> Y \<Longrightarrow> h (g X) \<equiv> g (h Y)"
+  sorry
 
 ML\<open>
-  single_pos @{context} hint_unif ""
-    (@{term_pat "id 5 ::nat"},
-     @{term_pat "Suc (Suc 5)"})\<close>
+  val (t1,t2) = (@{term_pat "h (g (f a))"},@{term_pat "g (h (f b))"});
+  single_pos (ctxt ()) hint_unif "" (t1,t2);
+\<close>
 
 ML\<open>
-  single_pos @{context} hint_unif ""
-    (@{term_pat "r ((id 5) + (2 - Suc (id ?Y)) = Suc 4)::nat"},
-     @{term_pat "(id r) (5 = id (Suc 4))::nat"})\<close>
+  val (t1,t2) = (@{term_pat "id (id 2) ::nat"}, @{term_pat "Suc ?x ::nat"});
+  single_pos (ctxt ()) hint_unif "" (t1,t2);
+\<close>
+
+consts r :: "nat \<Rightarrow> nat" t :: "nat \<Rightarrow> nat"
+
+(*recursive calls with alternating hints*)
+lemma [hints]:"X \<equiv> Y \<Longrightarrow> f X \<equiv> g Y"
+  sorry
+
+lemma [hints]:"X \<equiv> Y \<Longrightarrow> f2 X \<equiv> g2 Y"
+  sorry
+
+ML\<open>
+  val (t1,t2) = (@{term_pat "f2 (f (g 0)) ::nat"}, @{term_pat "g2 (f (g 0)) ::nat"});
+  single_pos (ctxt ()) hint_unif "" (t1,t2)\<close>
+
+(*premise order*)
+lemma h1[hints]: "Y \<equiv> f \<Longrightarrow> X \<equiv> Y a \<Longrightarrow> X \<equiv> Y b"
+sorry
+
+ML\<open>
+  val (t1,t2) = (@{term_pat "?g a ::nat"}, @{term_pat "?g b ::nat"});
+  single_pos (ctxt ()) hint_unif "" (t1,t2);
+  val (env,thm) = hint_unif (ctxt ()) (t1,t2) (Envir.empty 0);
+  pretty_env @{context} (Envir.term_env env);
+  pretty_thm @{context} thm |> pwriteln
+\<close>
+(*weiteres beispiel*)
+
 
 end
